More on countability.

theories/structure/Discrete.ec
@@ -26,67 +26,7 @@ op countable ['a] (E : 'a -> bool) =
   exists (C : int -> 'a option),
     forall x, E x => exists i, C i = Some x.
 
-(* -------------------------------------------------------------------- *)
-lemma L (n1 p1 n2 p2 : int) :
-     0 <= n1 => 0 <= p1
-  => 0 <= n2 => 0 <= p2
-  => exp 2 n1 * exp 3 p1 = exp 2 n2 * exp 3 p2
-  => n1 = n2 /\ p1 = p2.
-proof.
-move=> ge0_n1 ge0_p1 ge0_n2 ge0_p2; case: (n1 = n2) => /= [<-|neq_n].
-(* FIXME: move/ieexprIn fails *)
-+ have h/h{h} := mulfI (exp 2 n1) _; 1: by rewrite expf_eq0 //.
-  by have h := ieexprIn 3 _ _ p1 p2 _ _ => //; apply/ltzW.
-pose x1 := exp 3 p1; pose x2 := exp 3 p2.
-have {ge0_p1 ge0_p2} [o1 o2] : odd x1 /\ odd x2 by rewrite !oddX // odd3.
-(* FIXME: wlog *)
-(* FIXME: display of pose is not well indented *)
-pose P n1 n2 x1 x2 :=
-     0 <= n1 => 0 <= n2 => n1 <> n2 => odd x1 => odd x2
-  => exp 2 n1 * x1 <> exp 2 n2 * x2.
-move: x1 x2 ge0_n1 ge0_n2 neq_n o1 o2.
-move=> {p1 p2} x1 x2; rewrite -/(P n1 n2 x1 x2).
-have: (forall n1 n2 x1 x2, (n1 <= n2)%Int => P n1 n2 x1 x2) => P n1 n2 x1 x2.
-+ move=> ih; case: (lez_total n1 n2); first by move/ih; apply.
-  by move=> h @/P *; rewrite eq_sym &(ih) 1?eq_sym.
-apply=> {n1 n2 x1 x2} n1 n2 x1 x2 le_n ge0_n1 ge0_n2 neq_n o1 o2.
-have lt_n: n1 < n2 by rewrite ltr_neqAle le_n.
-rewrite (_ : n2 = n1 + (n2 - n1)) 1:#ring exprD ?subr_ge0 //.
-apply/negP; rewrite -mulrA; have h/h := mulfI (exp 2 n1) _.
-+ by rewrite expf_eq0.
-by move/(congr1 odd); rewrite oddM poddX ?subr_gt0 // odd2 !(o1, o2).
-qed.
-
-(* -------------------------------------------------------------------- *)
-lemma L (n1 p1 n2 p2 : int) :
-     0 < n1 => 0 < p1
-  => 0 < n2 => 0 < p2
-  => exp 2 n1 * exp 3 p1 = exp 2 n2 * exp 3 p2
-  => n1 = n2 /\ p1 = p2.
-proof.
-move=> gt0_n1 gt0_p1 gt0_n2 gt0_p2; case: (n1 = n2) => /= [<-|neq_n].
-(* FIXME: move/ieexprIn fails *)
-+ have h/h{h} := mulfI (exp 2 n1) _; 1: by rewrite expf_eq0 //.
-  by have h := ieexprIn 3 _ _ p1 p2 _ _ => //; apply/ltzW.
-pose x1 := exp 3 p1; pose x2 := exp 3 p2.
-have {gt0_p1 gt0_p2} [o1 o2] : odd x1 /\ odd x2 by rewrite !oddX // odd3.
-(* FIXME: wlog *)
-(* FIXME: display of pose is not well indented *)
-pose P n1 n2 x1 x2 :=
-     0 < n1 => 0 < n2 => n1 <> n2 => odd x1 => odd x2
-  => exp 2 n1 * x1 <> exp 2 n2 * x2.
-move: x1 x2 gt0_n1 gt0_n2 neq_n o1 o2.
-move=> {p1 p2} x1 x2; rewrite -/(P n1 n2 x1 x2).
-have: (forall n1 n2 x1 x2, (n1 <= n2)%Int => P n1 n2 x1 x2) => P n1 n2 x1 x2.
-+ move=> ih; case: (lez_total n1 n2); first by move/ih; apply.
-  by move=> h @/P *; rewrite eq_sym &(ih) 1?eq_sym.
-apply=> {n1 n2 x1 x2} n1 n2 x1 x2 le_n gt0_n1 gt0_n2 neq_n o1 o2.
-have lt_n: n1 < n2 by rewrite ltr_neqAle le_n.
-rewrite (_ : n2 = n1 + (n2 - n1)) 1:#ring exprD ?subr_ge0 1?ltrW //.
-apply/negP; rewrite -mulrA; have h/h := mulfI (exp 2 n1) _.
-+ by rewrite expf_eq0.
-by move/(congr1 odd); rewrite oddM oddX ?subr_gt0 // odd2 !(o1, o2).
-qed.
+abbrev countableT ['a] = countable predT<:'a>.
 
 (* -------------------------------------------------------------------- *)
 lemma nosmt inj_countable ['a] (f : 'a -> int) (p : 'a -> bool) :
@@ -98,6 +38,183 @@ pose C i := Some (choiceb (P i) witness).
 exists C => x px @/C; exists (f x); congr.
 have: exists y, P (f x) y by exists x.
 by case/(choicebP (P (f x)) witness)=> h; apply/inj_pf.
+qed.
+
+(* -------------------------------------------------------------------- *)
+lemma nosmt inj_cond_countable ['a 'b] (f : 'a -> 'b) pb pa :
+     countable<:'b> pb
+  => (forall x y, pa x => pa y => f x = f y => x = y)
+  => (forall x, pa x => pb (f x))
+  => countable<:'a> pa.
+proof. admitted.
+
+(* -------------------------------------------------------------------- *)
+lemma nosmt inj_condL_countable ['a 'b] (f : 'a -> 'b) p :
+     countableT<:'b>
+  => (forall x y, p x => p y => f x = f y => x = y)
+  => countable<:'a> p.
+proof. by apply/inj_cond_countable. qed.
+
+(* -------------------------------------------------------------------- *)
+lemma nosmt countable_inj ['a] (p : 'a -> bool) :
+  countable p => exists (f : 'a -> int), (* FIXME: (...) should not be mandatory *)
+    forall x y, p x => p y => f x = f y => x = y.
+proof.
+case=> C hC; exists (fun x => choiceb (fun i => C i = Some x) 0) => /=.
+move=> x y px py; have hx := hC x px; have hy := hC y py => {hC px py} h.
+have /= := choicebP _ 0 hy; have /= := choicebP _ 0 hx => {hx hy}.
+by rewrite -h => ->.
+qed.
+
+(* -------------------------------------------------------------------- *)
+op int2nat (i : int) : int =
+  if 0 <= i then 2 * i else -2 * i + 1.
+
+lemma inj_int2nat : injective int2nat.
+proof.
+move=> x y @/int2nat; case: (0 <= y); case: (0 <= x) => hx hy.
++ by apply: mulfI.
++ by move/(congr1 odd); rewrite oddS oddN !oddM odd2.
++ by move/(congr1 odd); rewrite oddS oddN !oddM odd2.
++ by move/addIr; rewrite -!mulNr &(mulfI) oppr_eq0.
+qed.
+
+lemma ge0_inj2nat x : 0 <= int2nat x by smt().
+
+(* -------------------------------------------------------------------- *)
+theory IntPair.
+  lemma FTA23 (n1 p1 n2 p2 : int) :
+       0 <= n1 => 0 <= p1
+    => 0 <= n2 => 0 <= p2
+    => exp 2 n1 * exp 3 p1 = exp 2 n2 * exp 3 p2
+    => n1 = n2 /\ p1 = p2.
+  proof.
+  move=> ge0_n1 ge0_p1 ge0_n2 ge0_p2; case: (n1 = n2) => /= [<-|neq_n].
+  (* FIXME: move/ieexprIn fails *)
+  + have h/h{h} := mulfI (exp 2 n1) _; 1: by rewrite expf_eq0 //.
+    by have h := ieexprIn 3 _ _ p1 p2 _ _ => //; apply/ltzW.
+  pose x1 := exp 3 p1; pose x2 := exp 3 p2.
+  have {ge0_p1 ge0_p2} [o1 o2] : odd x1 /\ odd x2 by rewrite !oddX // odd3.
+  (* FIXME: wlog *)
+  (* FIXME: display of pose is not well indented *)
+  pose P n1 n2 x1 x2 :=
+       0 <= n1 => 0 <= n2 => n1 <> n2 => odd x1 => odd x2
+    => exp 2 n1 * x1 <> exp 2 n2 * x2.
+  move: x1 x2 ge0_n1 ge0_n2 neq_n o1 o2.
+  move=> {p1 p2} x1 x2; rewrite -/(P n1 n2 x1 x2).
+  have: (forall n1 n2 x1 x2, (n1 <= n2)%Int => P n1 n2 x1 x2) => P n1 n2 x1 x2.
+  + move=> ih; case: (lez_total n1 n2); first by move/ih; apply.
+    by move=> h @/P *; rewrite eq_sym &(ih) 1?eq_sym.
+  apply=> {n1 n2 x1 x2} n1 n2 x1 x2 le_n ge0_n1 ge0_n2 neq_n o1 o2.
+  have lt_n: n1 < n2 by rewrite ltr_neqAle le_n.
+  rewrite (_ : n2 = n1 + (n2 - n1)) 1:#ring exprD ?subr_ge0 //.
+  apply/negP; rewrite -mulrA; have h/h := mulfI (exp 2 n1) _.
+  + by rewrite expf_eq0.
+  by move/(congr1 odd); rewrite oddM poddX ?subr_gt0 // odd2 !(o1, o2).
+  qed.
+
+  op encode (xy : int * int) =
+    exp 2 (int2nat xy.`1) * exp 3 (int2nat xy.`2).
+
+  lemma inj_encode : injective encode.
+  proof.
+  case=> [x1 y1] [x2 y2] @/encode /=; rewrite andabP.
+  rewrite -(inj_eq _ inj_int2nat x1) -(inj_eq _ inj_int2nat y1).
+  by apply/FTA23; apply/ge0_inj2nat.
+  qed.
+
+  lemma countable : countableT<:int * int>.
+  (* FIXME: type argument of countableT not shown *)
+  proof.
+  by apply/(@inj_countable encode)=> xy1 xy2 _ _; apply/inj_encode.
+  qed.
+end IntPair.
+
+(* -------------------------------------------------------------------- *)
+theory IntTuple.
+  op encode (s : int list) =
+    with s = []     => 0
+    with s = x :: s => IntPair.encode (x, encode s).
+
+  lemma inj_encode s1 s2 :
+    size s1 = size s2 => encode s1 = encode s2 => s1 = s2.
+  proof.
+  elim: s1 s2 => [|x1 s1 ih] [|x2 s2] //=; try by rewrite addz_neq0 ?size_ge0.
+  by move/addzI => /ih {ih}ih /IntPair.inj_encode [-> /ih ->].
+  qed.
+
+  lemma countable n : countable<:int list> (fun s => size s = n).
+  proof.
+  by apply/(@inj_countable encode) => /= s1 s2 <- /eq_sym; apply/inj_encode.
+  qed.
+end IntTuple.
+
+(* -------------------------------------------------------------------- *)
+theory IntList.
+  op encode (s : int list) =
+    IntPair.encode (size s, IntTuple.encode s).
+
+  lemma inj_encode : injective encode.
+  proof.
+  (* FIXME: unfolding encode should not be necessary *)
+  (* FIXME: unfolding encode should not unfold IntPair.encode *)
+  move=> s1 s2 @/IntList.encode /IntPair.inj_encode [].
+  by apply/IntTuple.inj_encode.
+  qed.
+
+  lemma countable : countableT<:int list>.
+  proof.
+  by apply/(@inj_countable encode)=> s1 s2 _ _; apply/inj_encode.
+  qed.
+end IntList.
+
+(* -------------------------------------------------------------------- *)
+lemma cnt_unit p : countable<:unit> p.
+proof. by apply/(@inj_countable (fun _ => 0)). qed.
+
+(* -------------------------------------------------------------------- *)
+lemma cnt_bool p : countable<:bool> p.
+proof. by apply/(@inj_countable b2i) => -[] -[]. qed.
+
+(* -------------------------------------------------------------------- *)
+lemma cnt_prod_cond ['a 'b] pa pb :
+     countable<:'a> pa
+  => countable <:'b> pb
+  => countable (fun (xy : _ * _) => pa xy.`1 /\ pb xy.`2).
+proof.
+case/countable_inj=> CA hA; case/countable_inj=> CB hB.
+pose f (xy : _ * _) := (CA xy.`1, CB xy.`2).
+apply/(@inj_condL_countable f) => /=; 1: by apply/IntPair.countable.
+case=> [x1 x2] [y1 y2] /= [hax hbx] [hay hby] [] /= hx hy.
+by rewrite (hA _ _ hax hay) // (hB _ _ hbx hby).
+qed.
+
+(* -------------------------------------------------------------------- *)
+lemma cnt_prod ['a 'b] :
+  countableT<:'a> => countableT<:'b> => countableT<:'a * 'b>.
+proof. by apply/cnt_prod_cond. qed.
+
+(* -------------------------------------------------------------------- *)
+lemma cnt_list_cond ['a] (p : 'a -> bool) :
+  countable p => countable (all p).
+proof.
+case/countable_inj=> C h; pose f s := map C s.
+apply/(@inj_condL_countable f); 1: by apply/IntList.countable.
+by apply/in_inj_map.
+qed.
+
+(* -------------------------------------------------------------------- *)
+lemma cnt_list ['a] : countableT<:'a> => countableT<:'a list>.
+proof.
+move/cnt_list_cond; suff ->//: all predT<:'a> = predT.
+by apply/fun_ext=> s; rewrite all_predT.
+qed.
+
+(* -------------------------------------------------------------------- *)
+lemma cnt_option ['a] : countableT<:'a> => countableT<:'a option>.
+proof.
+move=> h; pose f x := odflt [] (omap (fun y => [<:'a> y]) x).
+by apply(@inj_condL_countable f) => [|[|x] [|y]] //; apply/cnt_list.
 qed.
 
 (* -------------------------------------------------------------------- *)
